@prefix : <https://cogito.iot.linkeddata.es/def/resource#> .
@prefix owl: <http://www.w3.org/2002/07/owl#> .
@prefix rdf: <http://www.w3.org/1999/02/22-rdf-syntax-ns#> .
@prefix xml: <http://www.w3.org/XML/1998/namespace> .
@prefix xsd: <http://www.w3.org/2001/XMLSchema#> .
@prefix rdfs: <http://www.w3.org/2000/01/rdf-schema#> .
@base <https://cogito.iot.linkeddata.es/def/resource#> .

<https://cogito.iot.linkeddata.es/def/resource#> rdf:type owl:Ontology ;
                                                  <http://purl.org/dc/elements/1.1/creator> "María Poveda Villalón" ,
                                                                                            "Raúl García Castro" ,
                                                                                            "Socorro  Bernardos Galindo" ;
                                                  <http://purl.org/dc/elements/1.1/description> "The COGITO Resource ontology aims at modelling resources in the construction domain." ;
                                                  <http://purl.org/dc/elements/1.1/title> "Resource ontology" ;
                                                  <http://purl.org/dc/terms/license> <http://purl.org/NET/rdflicense/cc-by4.0> ;
                                                  owl:versionInfo "0.7.0" .

#################################################################
#    Annotation properties
#################################################################

###  http://purl.org/dc/elements/1.1/creator
<http://purl.org/dc/elements/1.1/creator> rdf:type owl:AnnotationProperty .


###  http://purl.org/dc/elements/1.1/description
<http://purl.org/dc/elements/1.1/description> rdf:type owl:AnnotationProperty .


###  http://purl.org/dc/elements/1.1/title
<http://purl.org/dc/elements/1.1/title> rdf:type owl:AnnotationProperty .


###  http://purl.org/dc/terms/license
<http://purl.org/dc/terms/license> rdf:type owl:AnnotationProperty .


#################################################################
#    Object Properties
#################################################################

###  https://cogito.iot.linkeddata.es/def/resource#belongsToType
:belongsToType rdf:type owl:ObjectProperty ;
               rdfs:range :ResourceType ;
               rdfs:comment "A property that relates an entity (especilly a resource:Resource) to its resource:ResourceType" ;
               rdfs:label "belongs to type" .


###  https://cogito.iot.linkeddata.es/def/resource#hasTackingTag
:hasTackingTag rdf:type owl:ObjectProperty ;
               rdfs:range <https://cogito.iot.linkeddata.es/def/iot#TrackingTag> ;
               rdfs:comment "A property that relates an entity (especilly a resource:Resource) to its iot:TrackingTag" ;
               rdfs:label "has tracking tag" .


#################################################################
#    Data properties
#################################################################

###  http://purl.org/dc/terms/identifier
<http://purl.org/dc/terms/identifier> rdf:type owl:DatatypeProperty ;
                                      rdfs:isDefinedBy <http://purl.org/dc/terms/> ;
                                      rdfs:label "identifier" .


###  http://purl.org/dc/terms/title
<http://purl.org/dc/terms/title> rdf:type owl:DatatypeProperty ;
                                 rdfs:isDefinedBy <http://purl.org/dc/terms/> ;
                                 rdfs:label "title" .


###  https://cogito.iot.linkeddata.es/def/resource#costPerHour
:costPerHour rdf:type owl:DatatypeProperty ;
             rdfs:comment "Property indicating the cost per hour of an entity (especially a resource:ResourceType)" ;
             rdfs:label "cost per hour" .


###  https://cogito.iot.linkeddata.es/def/resource#email
:email rdf:type owl:DatatypeProperty ;
       rdfs:comment "Property indicating the email of an entity (especially a resource:Worker)" ;
       rdfs:label "email" .


###  https://cogito.iot.linkeddata.es/def/resource#firstName
:firstName rdf:type owl:DatatypeProperty ;
           rdfs:comment "Property indicating the first name of an entity (especially a resource:Worker)" ;
           rdfs:label "first name" .


###  https://cogito.iot.linkeddata.es/def/resource#lastName
:lastName rdf:type owl:DatatypeProperty ;
          rdfs:comment "Property indicating the last name of an entity (especially a resource:Worker)" ;
          rdfs:label "last name" .


###  https://cogito.iot.linkeddata.es/def/resource#maxUnit
:maxUnit rdf:type owl:DatatypeProperty ;
         rdfs:comment "Property indicating the maximum number of units of an entity (especially a resource:ResourceType)" ;
         rdfs:label "maximum number of units" .


###  https://cogito.iot.linkeddata.es/def/resource#status
:status rdf:type owl:DatatypeProperty ;
        rdfs:comment "Property indicating the status of an entity (especially a resource:Resource)" ;
        rdfs:label "status" .


#################################################################
#    Classes
#################################################################

###  http://www.opengis.net/ont/geosparql#SpatialObject
<http://www.opengis.net/ont/geosparql#SpatialObject> rdf:type owl:Class ;
                                                     rdfs:isDefinedBy <http://www.opengis.net/ont/geosparql#> ;
                                                     rdfs:label "Spatial Object" .


###  https://cogito.iot.linkeddata.es/def/iot#TrackingTag
<https://cogito.iot.linkeddata.es/def/iot#TrackingTag> rdf:type owl:Class ;
                                                       rdfs:comment "A subclass of saref:Device and, as such, a tangible object designed to accomplish a particular task; in this case signalling its location" ;
                                                       rdfs:label "Tracking Tag" .


###  https://cogito.iot.linkeddata.es/def/resource#Equipment
:Equipment rdf:type owl:Class ;
           rdfs:subClassOf :Resource ;
           rdfs:comment "A subclass of resource:Resource used to assist in the performance of an activity (especially a process:Task)" ;
           rdfs:label "Equipment" .


###  https://cogito.iot.linkeddata.es/def/resource#EquipmentType
:EquipmentType rdf:type owl:Class ;
               rdfs:subClassOf :ResourceType ;
               rdfs:comment "The different kinds of (construction) equipment" ;
               rdfs:label "Equipment Type" .


###  https://cogito.iot.linkeddata.es/def/resource#Resource
:Resource rdf:type owl:Class ;
          rdfs:subClassOf <http://www.opengis.net/ont/geosparql#SpatialObject> ,
                          <https://saref.etsi.org/core#FeatureOfInterest> ;
          rdfs:comment "A source of supply, support, or aid, especially one that can be readily drawn upon when needed; and from which a property is measured" ;
          rdfs:label "Resource" .


###  https://cogito.iot.linkeddata.es/def/resource#ResourceType
:ResourceType rdf:type owl:Class ;
              rdfs:comment "The kind of resources assigned to a process:Task or involved in a process:Process" ;
              rdfs:label "Resource Type" .


###  https://cogito.iot.linkeddata.es/def/resource#Worker
:Worker rdf:type owl:Class ;
        rdfs:subClassOf :Resource ;
        rdfs:comment "A human resource that works in a project (especially performing a process:Task)" ;
        rdfs:label "Worker" .


###  https://cogito.iot.linkeddata.es/def/resource#WorkerRole
:WorkerRole rdf:type owl:Class ;
            rdfs:subClassOf :ResourceType ;
            rdfs:comment "The different kinds of roles a human worker can play in a (construction) project" ;
            rdfs:label "Worker Role" .


###  https://saref.etsi.org/core#FeatureOfInterest
<https://saref.etsi.org/core#FeatureOfInterest> rdf:type owl:Class ;
                                                rdfs:isDefinedBy <https://saref.etsi.org/core#> ;
                                                rdfs:label "Feature of Interest" .


###  Generated by the OWL API (version 5.1.14) https://github.com/owlcs/owlapi/
