<?xml version="1.0"?>
<rdf:RDF xmlns="https://cogito.iot.linkeddata.es/def/resource#"
     xml:base="https://cogito.iot.linkeddata.es/def/resource"
     xmlns:dc="http://purl.org/dc/elements/1.1/"
     xmlns:owl="http://www.w3.org/2002/07/owl#"
     xmlns:rdf="http://www.w3.org/1999/02/22-rdf-syntax-ns#"
     xmlns:xml="http://www.w3.org/XML/1998/namespace"
     xmlns:xsd="http://www.w3.org/2001/XMLSchema#"
     xmlns:rdfs="http://www.w3.org/2000/01/rdf-schema#"
     xmlns:terms="http://purl.org/dc/terms/">
    <owl:Ontology rdf:about="https://cogito.iot.linkeddata.es/def/resource#">
        <dc:creator>María Poveda Villalón</dc:creator>
        <dc:creator>Raúl García Castro</dc:creator>
        <dc:creator>Socorro  Bernardos Galindo</dc:creator>
        <dc:description>The COGITO Resource ontology aims at modelling resources in the construction domain.</dc:description>
        <dc:title>Resource ontology</dc:title>
        <terms:license rdf:resource="http://purl.org/NET/rdflicense/cc-by4.0"/>
        <owl:versionInfo>0.7.0</owl:versionInfo>
    </owl:Ontology>
    


    <!-- 
    ///////////////////////////////////////////////////////////////////////////////////////
    //
    // Annotation properties
    //
    ///////////////////////////////////////////////////////////////////////////////////////
     -->


    


    <!-- http://purl.org/dc/elements/1.1/creator -->


    <owl:AnnotationProperty rdf:about="http://purl.org/dc/elements/1.1/creator"/>
    


    <!-- http://purl.org/dc/elements/1.1/description -->


    <owl:AnnotationProperty rdf:about="http://purl.org/dc/elements/1.1/description"/>
    


    <!-- http://purl.org/dc/elements/1.1/title -->


    <owl:AnnotationProperty rdf:about="http://purl.org/dc/elements/1.1/title"/>
    


    <!-- http://purl.org/dc/terms/license -->


    <owl:AnnotationProperty rdf:about="http://purl.org/dc/terms/license"/>
    


    <!-- 
    ///////////////////////////////////////////////////////////////////////////////////////
    //
    // Object Properties
    //
    ///////////////////////////////////////////////////////////////////////////////////////
     -->


    


    <!-- https://cogito.iot.linkeddata.es/def/resource#belongsToType -->


    <owl:ObjectProperty rdf:about="https://cogito.iot.linkeddata.es/def/resource#belongsToType">
        <rdfs:range rdf:resource="https://cogito.iot.linkeddata.es/def/resource#ResourceType"/>
        <rdfs:comment>A property that relates an entity (especilly a resource:Resource) to its resource:ResourceType</rdfs:comment>
        <rdfs:label>belongs to type</rdfs:label>
    </owl:ObjectProperty>
    


    <!-- https://cogito.iot.linkeddata.es/def/resource#hasTackingTag -->


    <owl:ObjectProperty rdf:about="https://cogito.iot.linkeddata.es/def/resource#hasTackingTag">
        <rdfs:range rdf:resource="https://cogito.iot.linkeddata.es/def/iot#TrackingTag"/>
        <rdfs:comment>A property that relates an entity (especilly a resource:Resource) to its iot:TrackingTag</rdfs:comment>
        <rdfs:label>has tracking tag</rdfs:label>
    </owl:ObjectProperty>
    


    <!-- 
    ///////////////////////////////////////////////////////////////////////////////////////
    //
    // Data properties
    //
    ///////////////////////////////////////////////////////////////////////////////////////
     -->


    


    <!-- http://purl.org/dc/terms/identifier -->


    <owl:DatatypeProperty rdf:about="http://purl.org/dc/terms/identifier">
        <rdfs:isDefinedBy rdf:resource="http://purl.org/dc/terms/"/>
        <rdfs:label>identifier</rdfs:label>
    </owl:DatatypeProperty>
    


    <!-- http://purl.org/dc/terms/title -->


    <owl:DatatypeProperty rdf:about="http://purl.org/dc/terms/title">
        <rdfs:isDefinedBy rdf:resource="http://purl.org/dc/terms/"/>
        <rdfs:label>title</rdfs:label>
    </owl:DatatypeProperty>
    


    <!-- https://cogito.iot.linkeddata.es/def/resource#costPerHour -->


    <owl:DatatypeProperty rdf:about="https://cogito.iot.linkeddata.es/def/resource#costPerHour">
        <rdfs:comment>Property indicating the cost per hour of an entity (especially a resource:ResourceType)</rdfs:comment>
        <rdfs:label>cost per hour</rdfs:label>
    </owl:DatatypeProperty>
    


    <!-- https://cogito.iot.linkeddata.es/def/resource#email -->


    <owl:DatatypeProperty rdf:about="https://cogito.iot.linkeddata.es/def/resource#email">
        <rdfs:comment>Property indicating the email of an entity (especially a resource:Worker)</rdfs:comment>
        <rdfs:label>email</rdfs:label>
    </owl:DatatypeProperty>
    


    <!-- https://cogito.iot.linkeddata.es/def/resource#firstName -->


    <owl:DatatypeProperty rdf:about="https://cogito.iot.linkeddata.es/def/resource#firstName">
        <rdfs:comment>Property indicating the first name of an entity (especially a resource:Worker)</rdfs:comment>
        <rdfs:label>first name</rdfs:label>
    </owl:DatatypeProperty>
    


    <!-- https://cogito.iot.linkeddata.es/def/resource#lastName -->


    <owl:DatatypeProperty rdf:about="https://cogito.iot.linkeddata.es/def/resource#lastName">
        <rdfs:comment>Property indicating the last name of an entity (especially a resource:Worker)</rdfs:comment>
        <rdfs:label>last name</rdfs:label>
    </owl:DatatypeProperty>
    


    <!-- https://cogito.iot.linkeddata.es/def/resource#maxUnit -->


    <owl:DatatypeProperty rdf:about="https://cogito.iot.linkeddata.es/def/resource#maxUnit">
        <rdfs:comment>Property indicating the maximum number of units of an entity (especially a resource:ResourceType)</rdfs:comment>
        <rdfs:label>maximum number of units</rdfs:label>
    </owl:DatatypeProperty>
    


    <!-- https://cogito.iot.linkeddata.es/def/resource#status -->


    <owl:DatatypeProperty rdf:about="https://cogito.iot.linkeddata.es/def/resource#status">
        <rdfs:comment>Property indicating the status of an entity (especially a resource:Resource)</rdfs:comment>
        <rdfs:label>status</rdfs:label>
    </owl:DatatypeProperty>
    


    <!-- 
    ///////////////////////////////////////////////////////////////////////////////////////
    //
    // Classes
    //
    ///////////////////////////////////////////////////////////////////////////////////////
     -->


    


    <!-- http://www.opengis.net/ont/geosparql#SpatialObject -->


    <owl:Class rdf:about="http://www.opengis.net/ont/geosparql#SpatialObject">
        <rdfs:isDefinedBy rdf:resource="http://www.opengis.net/ont/geosparql#"/>
        <rdfs:label>Spatial Object</rdfs:label>
    </owl:Class>
    


    <!-- https://cogito.iot.linkeddata.es/def/iot#TrackingTag -->


    <owl:Class rdf:about="https://cogito.iot.linkeddata.es/def/iot#TrackingTag">
        <rdfs:comment>A subclass of saref:Device and, as such, a tangible object designed to accomplish a particular task; in this case signalling its location</rdfs:comment>
        <rdfs:label>Tracking Tag</rdfs:label>
    </owl:Class>
    


    <!-- https://cogito.iot.linkeddata.es/def/resource#Equipment -->


    <owl:Class rdf:about="https://cogito.iot.linkeddata.es/def/resource#Equipment">
        <rdfs:subClassOf rdf:resource="https://cogito.iot.linkeddata.es/def/resource#Resource"/>
        <rdfs:comment>A subclass of resource:Resource used to assist in the performance of an activity (especially a process:Task)</rdfs:comment>
        <rdfs:label>Equipment</rdfs:label>
    </owl:Class>
    


    <!-- https://cogito.iot.linkeddata.es/def/resource#EquipmentType -->


    <owl:Class rdf:about="https://cogito.iot.linkeddata.es/def/resource#EquipmentType">
        <rdfs:subClassOf rdf:resource="https://cogito.iot.linkeddata.es/def/resource#ResourceType"/>
        <rdfs:comment>The different kinds of (construction) equipment</rdfs:comment>
        <rdfs:label>Equipment Type</rdfs:label>
    </owl:Class>
    


    <!-- https://cogito.iot.linkeddata.es/def/resource#Resource -->


    <owl:Class rdf:about="https://cogito.iot.linkeddata.es/def/resource#Resource">
        <rdfs:subClassOf rdf:resource="http://www.opengis.net/ont/geosparql#SpatialObject"/>
        <rdfs:subClassOf rdf:resource="https://saref.etsi.org/core#FeatureOfInterest"/>
        <rdfs:comment>A source of supply, support, or aid, especially one that can be readily drawn upon when needed; and from which a property is measured</rdfs:comment>
        <rdfs:label>Resource</rdfs:label>
    </owl:Class>
    


    <!-- https://cogito.iot.linkeddata.es/def/resource#ResourceType -->


    <owl:Class rdf:about="https://cogito.iot.linkeddata.es/def/resource#ResourceType">
        <rdfs:comment>The kind of resources assigned to a process:Task or involved in a process:Process</rdfs:comment>
        <rdfs:label>Resource Type</rdfs:label>
    </owl:Class>
    


    <!-- https://cogito.iot.linkeddata.es/def/resource#Worker -->


    <owl:Class rdf:about="https://cogito.iot.linkeddata.es/def/resource#Worker">
        <rdfs:subClassOf rdf:resource="https://cogito.iot.linkeddata.es/def/resource#Resource"/>
        <rdfs:comment>A human resource that works in a project (especially performing a process:Task)</rdfs:comment>
        <rdfs:label>Worker</rdfs:label>
    </owl:Class>
    


    <!-- https://cogito.iot.linkeddata.es/def/resource#WorkerRole -->


    <owl:Class rdf:about="https://cogito.iot.linkeddata.es/def/resource#WorkerRole">
        <rdfs:subClassOf rdf:resource="https://cogito.iot.linkeddata.es/def/resource#ResourceType"/>
        <rdfs:comment>The different kinds of roles a human worker can play in a (construction) project</rdfs:comment>
        <rdfs:label>Worker Role</rdfs:label>
    </owl:Class>
    


    <!-- https://saref.etsi.org/core#FeatureOfInterest -->


    <owl:Class rdf:about="https://saref.etsi.org/core#FeatureOfInterest">
        <rdfs:isDefinedBy rdf:resource="https://saref.etsi.org/core#"/>
        <rdfs:label>Feature of Interest</rdfs:label>
    </owl:Class>
</rdf:RDF>



<!-- Generated by the OWL API (version 5.1.14) https://github.com/owlcs/owlapi/ -->


